\documentclass[a4paper]{article}
\usepackage[english]{babel}
\usepackage[utf8]{inputenc}

% mathermatics
\usepackage[fleqn]{mathtools} % left aligned equations, comment out for centered
\DeclarePairedDelimiter{\ceil}{\lceil}{\rceil}
\usepackage{amsmath} % more useful math
\usepackage{amssymb} % useful math symbols

% graphics
\usepackage{graphicx}
\usepackage{float}    % for more accurate graphics placement
\usepackage{fancyhdr} % for top header

% formatting
\usepackage{enumitem} % provides easy change of labels in enumerate environment
\usepackage[top=3cm, bottom=4cm, width=17cm]{geometry} % for smaller page margins

% colors
\usepackage{xcolor}

%% coding
% 
% uncomment this after you have completed the required installation
% see https://github.com/gpoore/minted for info
%
%\usepackage{minted} 
%\definecolor{codeBgColor}{RGB}{240,240,240}
%



% very simple alias, \ex{} becomes the same as \subsubsection*{}
% TIP: remove the * in the line below if you want it numbered
\newcommand{\ex}[1]{\subsubsection*{#1}}

% macro for multiple lines of equations
% use \intertext{text} for text between equations
% always end equations with a linefeed: \\ 
\newcommand{\eqns}[1]{
    \begin{align}
        \begin{split} \nonumber
            #1
        \end{split}
    \end{align}
}




%Begining of the document
\begin{document}

\pagestyle{fancy} % use pagestyle with simple header (from fancyhdr)

%\pagenumbering{gobble} % uncomment to remove pagenumbering (in case of single page document)
\fancyhead[L]{TMA4140 Diskret Matematikk}
\fancyhead[C]{\textbf{Ã˜ving 2}}
\fancyhead[R]{Otto Lote 748704}


\vspace{2em}
\subsection*{Section 2.1}
\vspace{1em}

\ex{Exercise 5}
\( \forall x \big( x \in A \leftrightarrow x \in B  \big) \leftrightarrow A = B \)   
\begin{enumerate}[label=\alph*)]
    \item \( A = B \) since A contains all elements of B and vice versa

    \item \( ((1)) \in A \land ((1)) \in B \) but \( (1) \notin A \rightarrow A \neq B\) 

    \item \( \emptyset \) is an empty set, and is not equal to a set containing an empty set.
\end{enumerate}


\ex{Exercise 24}
\begin{enumerate}[label=\alph*)]
    \item No. The power set of a set always include a set of an empty set: 
        \( P(\emptyset) = (\emptyset) \) 
        meaning a power set of a set is never empty. 
        \( \forall A \big( (\emptyset) \in P(A)  \big) \rightarrow 
        P(A) \neq \emptyset\)

    \item Yes. \( P((a)) = (\emptyset, (a)) \)

    \item No. \( P((\emptyset, a)) = 
        \big(\emptyset, (a), (\emptyset), (a, \emptyset)\big) \)
        The set in question is missing a \((\emptyset)\)

    \item Yes. \( P((a, b)) = \big(\emptyset, (a), (b), (a,b)\big) \) 
\end{enumerate}



\vspace{2em}
\subsection*{Section 2.2}
\vspace{1em}

\ex{Exercise 18}
\begin{enumerate}[label=\alph*), start=3]
    \item{ 
        \( (A-B) \equiv \forall x \mid x \in A \land x \notin B \)

        \( (A-B) -C \equiv \forall x \mid x \in (A-B) \land x \notin C \)

        \( (A-B) -C \equiv \forall x \mid x \in A \land x \notin B \land x \notin C \)

        \( (A-C) \equiv \forall x \mid x \in A \land x \notin C \)

        Since all elements of \( (A-B)-C \) are in \( (A-C) \), 
            \( (A-B)-C \subseteq (A-C) \)
    }

    \item{ 
        \( (A-C) \equiv \forall x \mid x \in A \land x \notin C \)

        \( (C-B) \equiv \forall x \mid x \in C \land x \notin B \)

        \( (A-C) \cap (C-B) \equiv \forall x \mid x \in (A-C) \land x \in (C-B) \)

        \( (A-C) \cap (C-B) \equiv \forall x \mid (x \in A \land x \notin C) \land 
            (x \in C \land x \notin B) \)

        Rewriting the paranthesis we get 

        \( (A-C) \cap (C-B) \equiv \forall x \mid x \in A \land 
            \underbrace{(x \notin C \land x \in C)}_{x \in \emptyset} \land x \notin B \)

        Clearly, \( (A-C) \cap (C-B) = \emptyset \)

    }
\end{enumerate}


\ex{Exercise 46}
\begin{align}
    \begin{split} \nonumber 
        \intertext{The set \(A \cup B\) consists of all elements in A that are also in B.} 
        A \cup B &= \forall x \mid x \in A \land x \in B \\
        \intertext{Another way of describing \( A \cup B \) is to look at all elements in A plus all elements in B minus the duplicates, which are elements in both A and B.}
        |A \cup B| &= |A| + |B| - |A \cap B| \\
        \intertext{This also holds for \( A \cup B \cup C \) but this time we
        have more duplicates. Elements in \( A \cap B \), \( A \cap C \) and \(
        B \cap C \) are "counted" twice, and elements in \( A \cap B \cap C \)
        are "counted" an extra time. }
        |A \cup B \cup C| &= |A| + |B| + |C| - \underbrace{|A \cap B| - |A \cap C| - |B \cap C|}_{\text{elements covered twice by } |A|+|B|+|C|} - \underbrace{|A \cap B \cap C|}_{\text{elements covered three times by }|A|+|B|+|C|}
    \end{split}
\end{align}



\vspace{2em}
\subsection*{Section 2.3}
\vspace{1em}

\ex{Exercise 12}
\begin{enumerate}[label=\alph*)]
    \item \( f(n) = n-1 \) is one-to-one since the function is strictly
        growing. Since every \(\Delta n\) increase on its domain will produce a
        \(\Delta y\) increase on its codomain, all values of n maps to a unique
        value

    \item \( f(n) = n^2 + 1 \) is one-to-one since \(f: \mathbb{Z} \mapsto
        \mathbb{Z}\) and is strictly growing (even in n=0 because of
        \(\mathbb{Z}\)). 

    \item \( f(n) = n^3 \) is one to one for the same reason as in b)

    \item \( f(n) = \ceil{n/2} \) is not one to one since every value of n maps to two values (except for n = 0).
\end{enumerate}

\ex{Exercise 38}
\eqns{
        f(x) &= ax+b \\
        g(x) &= cx+d \\
        f \circ g &= f(g(x)) = a(cx+d)+b = acx + ad + b \\
        g \circ f &= g(f(x)) = c(ax+b)+d = acx + cb + d \\
        f \circ g &= g \circ f \iff ad + b = cb + d
}


\ex{Exercise 42}
\( f:\mathbb{R} \mapsto \mathbb{R} \) given by \( f(x) = x^2 \) has an inverse
    \(f^{-1}\) given by \( f^{-1}(x) = \pm \sqrt{x}\)
\begin{enumerate}[label=\alph*)]
    \item \( f^{-1} (\{1\}) = \pm 1\)

    \item \( f^{-1} (\{ x \mid 0 < x < 1\}) = \pm\{ x \mid 0 < x < \sqrt{1} \}
        = \{ x \mid -1 < x < 1 \underbrace{\land x \neq 0}_{\text{input not
        defined for \(x = 0\)}} \}\)

    \item \( f^{-1} ( \{ x \mid x > 4 \} ) = \pm\{ x \mid x > \sqrt{4} \} 
        = \{ x \mid -2 > x \land x > 2 \} \)
\end{enumerate}


\vspace{2em}
\subsection*{Section 2.4}
\vspace{1em}

\ex{Exercise 12}
\( a_n = -3a_{n-1} + 4a_{n-2} \)
\begin{enumerate}[label=\alph*)]
    \item{ \eqns{
            a_n = 0 \implies -3a_{n-1} + 4a_{n-2} = -3(0) + 4(0) = 0 = a_n\\
            \intertext{Which means \(a_n = 0\) is a trivial solution to the
            recurrence relation}
    } }

    \item{ \eqns{
            a_n = 1 \implies -3a_{n-1} + 4a_{n-2} = -3 + 4 = 1 = a_n\\
            \intertext{\(a_n = 1\) is a solution to the recurrence relation}
    } }

    \item{ \eqns {
            a_n = (-4)^n \implies -3a_{n-1} + 4a_{n-2} &= 
                -3((-4)^{n-1}) + 4((-4)^{n-2})  \\
            &= -3((-4)(-4)^{n-2}) + 4((-4)^{n-2}) \\
            \intertext{We pull \((-4)^{n-2}\) from the parentheses}
            &= (-4)^{n-2} (-3)((-4)) + (-4)^{n-2}4(1) ) \\
            &= (-4)^{n-2} ( (-3)(-4) + 4 ) \\
            &= (-4)^{n-2} (18) \neq a_n
            \intertext{\(a_n = (-4)^n\) is not a solution to the recurrence relation}
    } }

    \item   \eqns {
            a_n = 2(-4)^n + 3 \implies -3a_{n-1} + 4a_{n-2} &=
                -3\big( 2(-4)^{n-1} + 3 \big) + 4\big( 2(-4)^{n-2} + 3 \big) \\
            &= -6(-4)^{n-1} -9  +  8(-4)^{n-2} + 12  \\
            &= -6(-4)(-4)^{n-2} +  8(-4)^{n-2} + 3 \\
            &= 24(-4)^{n-2} +  8(-4)^{n-2} + 3  \\
            &= 32(-4)^{n-2} +  3  \\
            &= 2(-4)^2(-4)^{n-2} +  3  \\
            &= 2(-4)^n +  3 = a_n \\
            \intertext{\(a_n = 2(-4)^n + 3\) is a solution to the recurrence relation}
    }

\end{enumerate}


\ex{Exercise 33}
\begin{enumerate}[label=\alph*)]
    \item \eqns {
            \sum_{i=1}^2{\sum_{j=1}^{3}{(i+j)}} &= 
                \sum_{i=1}^2{ \big( 3i + \sum_{j=1}^3{ j } \big) }\\
            &= \sum_{i=1}^2{ (3i + 6) }\\
            &= 12 + \sum_{i=1}^2{ 3i  }\\
            &= 12 + 9 = 21\\
    }

    \item \eqns { 
            \sum_{i=0}^2{\sum_{j=0}^{3}{(2i+3j)}} &= 
                \sum_{i=0}^2{ \big( 8i + \sum_{j=0}^3{ 3j } \big) }\\
            &= \sum_{i=0}^2{ \big( 8i + 21 \big) }\\
            &= 63 + \sum_{i=0}^2{  8i  }\\
            &= 63 + 24 = 87\\
    }

    \item \eqns {
            \sum_{i=1}^3{\sum_{j=0}^{2}{i}} &= 
                \sum_{i=1}^3{ \big( 3i + \sum_{j=0}^2{ 0 } \big) }\\
            &= \sum_{i=1}^3{  3i  }\\
            &= 3 + 6 + 9 = 18
    }

    \item \eqns {
            \sum_{i=0}^2{ \sum_{j=1}^3{  ij  } } &= 
                \sum_{i=0}^2{ \big( i \sum_{j=1}^3{ j } \big) } \\
            &= \sum_{i=0}^2{ 6i  } \\
            &= 0 + 6 + 12 = 18
    }

\end{enumerate}


\vspace{2em}
\subsection*{Section 2.5}
\vspace{1em}

\ex{Exercise 16}
\begin{enumerate}[label=\alph*)]
    \item{
    }
\end{enumerate}


%% uncomment this if you need references. Edit the .bbl file with your references
%% and use "\cite{bibitem-label}" to cite
%\bibliography{template}

\end{document}

